src/tidy/monad_chain.2.lean
@@ -1,0 +1,38 @@
+import .if_then_else
+import .tidy
+
+universe variables u v w
+
+meta class tactical_monad (state : Type) [m : monad (interaction_monad state)] extends monad_fail (interaction_monad state), has_orelse (interaction_monad state) :=
+  ( lift : Π { α : Type u }, tactic α → (interaction_monad state) α )
+
+meta def failed {α : Type u} {state : Type} [tactical_monad state]: (interaction_monad state) α := monad_fail.fail (interaction_monad state) ""
+meta def fail   {α : Type u} {state : Type} [tactical_monad state] {β : Type u} [has_to_format β] (msg : β) : (interaction_monad state) α :=
+  monad_fail.fail (interaction_monad state) (to_fmt msg).to_string
+
+meta instance lift_tactic_coe {α : Type u} (state : Type) [m : monad (interaction_monad state)] [tm : @tactical_monad state m] : has_coe (tactic α) ((interaction_monad state) α) := ⟨ @tactical_monad.lift _ m tm _ ⟩
+
+meta instance trivial_tactical_monad : tactical_monad tactic_state := {
+  interaction_monad.monad with
+  fail   := λ { α : Type }, tactic.fail,
+  orelse := λ { α : Type }, interaction_monad_orelse,
+  lift   := λ { α : Type }, id
+}
+
+meta structure chain_progress {state : Type} (α : Type u) :=
+  ( iteration_limit   : nat )
+  ( results           : list α )
+  ( remaining_tactics : list ((interaction_monad state) α) )
+
+open nat tactic
+
+private meta def chain' {α : Type u} {state : Type} [tm : tactical_monad state] ( tactics : list ((interaction_monad state) α) ) 
+    : chain_progress α → (interaction_monad state) (list α)
+| ⟨ 0     , _      , _       ⟩ := fail "chain iteration limit exceeded"
+| ⟨ _     , results, []      ⟩ := pure results
+| ⟨ succ n, results, t :: ts ⟩ := if_then_else done
+                                   (pure results)
+                                   (dependent_if_then_else t 
+                                      (λ result, (chain' ⟨ n, result :: results, tactics ⟩ ))
+                                      (chain' ⟨ succ n, results, ts ⟩)
+)
